more for full GNF

Replace_Terminals.thy
@@ -6,6 +6,20 @@ begin
 lemma inj_on_cong2: "(\<And>a. a \<in> A \<Longrightarrow> f a = g a) \<Longrightarrow> A = B \<Longrightarrow> inj_on f A \<longleftrightarrow> inj_on g B"
   by (auto simp: inj_on_def)
 
+lemma Lhss_image_Pair: "Lhss ((\<lambda>x. (f x, g x)) ` X) = f ` X"
+  by (auto simp: Lhss_def)
+
+lemma Rhss_image_Pair_inj_on:
+  assumes f: "inj_on f X" and x: "x \<in> X"
+  shows "Rhss ((\<lambda>x. (f x, g x)) ` X) (f x) = {g x}"
+  using inj_onD[OF f] x by (auto simp: Rhss_def)
+
+lemma Lang_Un_disj_Lhss:
+  assumes disj: "Nts P \<inter> Lhss Q = {}" and A: "A \<in> Nts P"
+  shows "Lang (P \<union> Q) A = Lang P A"
+  sorry
+
+
 
 fun fresh_map :: "'a :: fresh0 set \<Rightarrow> 'b list \<Rightarrow> 'b \<Rightarrow> 'a" where
   "fresh_map A [] = undefined"
@@ -38,64 +52,57 @@ lemma fresh_map_distinct:
   shows "distinct (map (fresh_map A xs) xs) \<longleftrightarrow> distinct xs" (is "?l \<longleftrightarrow> ?r")
   using inj_on_fresh_map[OF fin] by (auto simp: distinct_map)
 
+definition Replace_grammar where
+"Replace_grammar f as = (\<lambda>a. (f a, [Tm a])) ` as"
+
 definition replace_grammar where
-"replace_grammar As as = [(fresh_map As as a, [Tm a]). a \<leftarrow> as]"
+"replace_grammar f as = [(f a, [Tm a]). a \<leftarrow> as]"
 
-lemma Lang_Un_replace_grammar:
-  assumes As: "Nts P \<subseteq> As" and A: "A \<in> Nts P"
-  shows "Lang (P \<union> set (replace_grammar As as)) A = Lang P A"
-  sorry
+lemma set_replace_grammar: "set (replace_grammar f as) = Replace_grammar f (set as)"
+  by (auto simp: replace_grammar_def Replace_grammar_def)
 
-lemma lhss_replace_grammar: "lhss (replace_grammar As as) = fresh_map As as ` set as"
-  by (auto simp: replace_grammar_def Lhss_def)
+lemma Lhss_Replace_grammar: "Lhss (Replace_grammar f as) = f ` as"
+  by (simp add: Replace_grammar_def Lhss_image_Pair)
 
-lemma rhss_replace_grammar:
-  assumes fin: "finite As" and a: "a \<in> set as"
-  shows "Rhss (set (replace_grammar As as)) (fresh_map As as a) = {[Tm a]}"
-  using inj_on_fresh_map[OF fin, of as, THEN inj_onD]
-  by (auto simp: replace_grammar_def Rhss_def a)
+lemma Rhss_Replace_grammar:
+  assumes inj: "inj_on f as" and a: "a \<in> as"
+  shows "Rhss (Replace_grammar f as) (f a) = {[Tm a]}"
+  by (auto simp: Replace_grammar_def Rhss_image_Pair_inj_on[OF inj a])
 
-lemma Rhss_Un_replace_grammar:
-  assumes fin: "finite As" and As: "Lhss P \<subseteq> As" and a: "a \<in> set as"
-  shows "Rhss (P \<union> set (replace_grammar As as)) (fresh_map As as a) = {[Tm a]}"
+lemma Rhss_Un_Replace_grammar:
+  assumes inj: "inj_on f as" and a: "a \<in> as" and fa: "f a \<notin> Lhss P"
+  shows "Rhss (P \<union> Replace_grammar f as) (f a) = {[Tm a]}"
+  by (simp add: Rhss_Un Rhss_Replace_grammar[OF inj a] fa[unfolded notin_Lhss_iff_Rhss])
+
+lemma Lang_Replace_grammar1:
+  assumes inj: "inj_on f as" and a: "a \<in> as"
+    and faP: "f a \<notin> Lhss P" and A: "A \<noteq> f a"
+  shows "Lang (insert (A, \<alpha> @ Nt (f a) # \<beta>) (P \<union> Replace_grammar f as)) =
+         Lang (insert (A, \<alpha> @ Tm a # \<beta>) (P \<union> Replace_grammar f as))"
 proof-
-  from As fresh_map_notIn[OF fin a]
-  have "fresh_map As as a \<notin> Lhss P" by auto
-  then show ?thesis
-    by (simp add: Rhss_Un rhss_replace_grammar[OF fin a] notin_Lhss_iff_Rhss)
-qed
-
-lemma Lang_replace_grammar1:
-  assumes fin: "finite As" and PAs: "Lhss P \<subseteq> As" and a: "a \<in> set as"
-    and AAs: "A \<in> As"
-  shows "Lang (insert (A, \<alpha> @ Nt (fresh_map As as a) # \<beta>) (P \<union> set (replace_grammar As as))) =
-         Lang (insert (A, \<alpha> @ Tm a # \<beta>) (P \<union> set (replace_grammar As as)))"
-proof-
-  note Rhss = Rhss_Un_replace_grammar[OF fin PAs a]
-  have neq: "A \<noteq> fresh_map As as a" using fresh_map_notIn[OF fin a] AAs by auto
-  note * = Lang_subst1[OF neq Rhss, where \<alpha> = \<alpha> and \<gamma> = \<beta>, simplified]
+  note Rhss = Rhss_Un_Replace_grammar[OF inj a faP]
+  note * = Lang_subst1[OF A Rhss, where \<alpha> = \<alpha> and \<gamma> = \<beta>, simplified]
   show ?thesis by (simp add: *)
 qed
 
 definition replace_sym where
-"replace_sym As as x = (case x of Tm a \<Rightarrow> Nt (fresh_map As as a) | _ \<Rightarrow> x)"
+"replace_sym f x = (case x of Tm a \<Rightarrow> Nt (f a) | _ \<Rightarrow> x)"
 
-lemma replace_sym_Nt: "replace_sym As as (Nt A) = Nt A"
-  and replace_sym_Tm: "replace_sym As as (Tm a) = Nt (fresh_map As as a)"
+lemma replace_sym_Nt: "replace_sym f (Nt A) = Nt A"
+  and replace_sym_Tm: "replace_sym f (Tm a) = Nt (f a)"
   by (auto simp: replace_sym_def)
 
-lemma Lang_replace_grammar_append:
-  assumes fin: "finite As" and PAs: "Lhss P \<subseteq> As" and Pas: "Tms P \<subseteq> set as"
-    and AAs: "A \<in> As"
-  shows "Tms_syms \<beta> \<subseteq> set as \<Longrightarrow>
- Lang (insert (A, \<alpha> @ map (replace_sym As as) \<beta>) (P \<union> set (replace_grammar As as))) =
- Lang (insert (A, \<alpha> @ \<beta>) (P \<union> set (replace_grammar As as)))"
+lemma Lang_Replace_grammar_append:
+  assumes inj: "inj_on f as" and Pfas: "Lhss P \<inter> f ` as = {}" and Afas: "A \<notin> f ` as"
+  defines "P' \<equiv> P \<union> Replace_grammar f as"
+  shows "Tms_syms \<beta> \<subseteq> as \<Longrightarrow>
+ Lang (insert (A, \<alpha> @ map (replace_sym f) \<beta>) P') = Lang (insert (A, \<alpha> @ \<beta>) P')"
 proof (induction \<beta> arbitrary: \<alpha>)
   case Nil
   show ?case by simp
 next
   case (Cons x \<beta>)
-  from Cons.prems have "Tms_syms \<beta> \<subseteq> set as" by auto
+  from Cons.prems have "Tms_syms \<beta> \<subseteq> as" by auto
   note IH = Cons.IH[OF this, where \<alpha> = "\<alpha> @ [x]"]
   show ?case
   proof (cases x)
@@ -103,10 +110,92 @@ next
     with IH show ?thesis by (auto simp: replace_sym_Nt)
   next
     case [simp]: (Tm a)
-    from Cons.prems have "a \<in> set as" by auto
-    note * = Lang_replace_grammar1[OF fin PAs this AAs]
-    from IH show ?thesis by (simp add: replace_sym_Tm *)
+    from Cons.prems have a: "a \<in> as" by auto
+    from a Pfas have fa: "f a \<notin> Lhss P" by auto
+    from a Afas have A: "A \<noteq> f a" by auto
+    note * = Lang_Replace_grammar1[OF inj a fa A]
+    from IH show ?thesis by (simp add: replace_sym_Tm * P'_def)
   qed
+qed
+
+definition map_tl where
+"map_tl f xs = (case xs of x#xs' \<Rightarrow> x # map f xs' | _ \<Rightarrow> xs)"
+
+lemma map_tl_simps[simp]:
+"map_tl f [] = []"
+"map_tl f (x#xs) = x # map f xs"
+  by (auto simp: map_tl_def)
+
+lemma Lang_map_tl_replace:
+  assumes pre: "inj_on f as" "Lhss P \<inter> f ` as = {}" "A \<notin> f ` as"
+    and \<alpha>: "Tms_syms \<alpha> \<subseteq> as"
+  defines "P' \<equiv> P \<union> Replace_grammar f as"
+  shows "Lang (insert (A, map_tl (replace_sym f) \<alpha>) P') = Lang (insert (A,\<alpha>) P')"
+proof (cases \<alpha>)
+  case Nil
+  then show ?thesis by simp
+next
+  case [simp]: (Cons x \<beta>)
+  with \<alpha> have \<beta>: "Tms_syms \<beta> \<subseteq> as" by simp
+  from Lang_Replace_grammar_append[OF pre \<beta>, where \<alpha> = "[x]"]
+  show ?thesis by (simp add: P'_def)
+qed
+
+definition replace_tl where
+"replace_tl f P = [(A, map_tl (replace_sym f) \<alpha>). (A,\<alpha>) \<leftarrow> P]"
+
+lemma "replace_tl f = map (map_prod id (map_tl (replace_sym f)))"
+  by (simp add: fun_eq_iff replace_tl_def split: prod.split)
+
+lemma replace_tl_simps[simp]:
+"replace_tl f [] = []"
+"replace_tl f ((A,\<alpha>)#P) = (A, map_tl (replace_sym f) \<alpha>) # replace_tl f P"
+  by (simp_all add: replace_tl_def)
+
+definition replace_Tm_tl where
+"replace_Tm_tl f P = replace_tl f P @ replace_grammar f (tms P)"
+
+lemma lang_replace_Tm_tl:
+  assumes inj: "inj_on f (Tms (set P))" and Nts: "Nts (set P) \<inter> f ` Tms (set P) = {}"
+    and A: "A \<in> Nts (set P)"
+  shows "lang (replace_Tm_tl f P) A = lang P A"
+proof-
+  have Lhss: "Lhss (set P) \<inter> f ` Tms (set P) = {}" using Nts by (auto simp: Nts_Lhss_Rhs_Nts)
+  { fix as
+    assume inj: "inj_on f as"
+      and Pfas: "Lhss (set P) \<inter> f ` as = {}"
+      and Pas: "Tms (set P) \<subseteq> as"
+    from Pfas Pas
+    have "\<And>Q. Lhss Q \<inter> f ` as = {} \<Longrightarrow> Lang (Q \<union> set (replace_tl f P) \<union> Replace_grammar f as) = Lang (Q \<union> set P \<union> Replace_grammar f as)"
+    proof (induction P)
+      case Nil
+      show ?case by simp
+    next
+      case (Cons p P)
+      show ?case
+      proof (cases p)
+        case [simp]: (Pair A \<alpha>)
+        from Cons
+        have Afas: "A \<notin> f ` as" and Pfas: "lhss P \<inter> f ` as = {}"
+          and Qfas: "Lhss Q \<inter> f ` as = {}"
+          and Pas: "Tms (set P) \<subseteq> as" and \<alpha>as: "Tms_syms \<alpha> \<subseteq> as"
+          by (auto simp: Tms_def)
+        from Afas Qfas have "Lhss (Q \<union> {(A,\<alpha>')}) \<inter> f ` as = {}" for \<alpha>' by (simp add: ac_simps)
+        note IH = Cons.IH[OF this Pfas Pas, simplified]
+        from Pfas Qfas have QPfas: "Lhss (Q \<union> set P) \<inter> f ` as = {}" by auto
+        from Lang_map_tl_replace[OF inj QPfas Afas \<alpha>as]
+        show ?thesis by (simp add: IH)
+      qed
+    qed
+  }
+  from this[of "set (tms P)" "{}",simplified] inj Lhss
+  have 1: "lang (replace_Tm_tl f P) = Lang (set P \<union> Replace_grammar f (Tms (set P)))"
+    by (simp add: replace_Tm_tl_def set_tms set_replace_grammar)
+  have 2: "\<dots> A = lang P A"
+    apply (subst Lang_Un_disj_Lhss[OF _ A])
+     apply (simp add: Lhss_Replace_grammar Nts) (* !? *)
+    apply (rule refl).
+  show ?thesis by (simp add: 1 2)
 qed
 
 
